@prefix : <http://www.semanticweb.org/mdebe/ontologies/2024/6/climatology/> .
@prefix owl: <http://www.w3.org/2002/07/owl#> .
@prefix rdf: <http://www.w3.org/1999/02/22-rdf-syntax-ns#> .
@prefix xml: <http://www.w3.org/XML/1998/namespace> .
@prefix xsd: <http://www.w3.org/2001/XMLSchema#> .
@prefix rdfs: <http://www.w3.org/2000/01/rdf-schema#> .
@base <http://www.semanticweb.org/mdebe/ontologies/2024/6/climatology/> .

<http://www.semanticweb.org/mdebe/ontologies/2024/6/climatology> rdf:type owl:Ontology ;
                                                                  rdfs:seeAlso <http://www.w3.org/TR/skos-reference/> ;
                                                                  <http://www.w3.org/2004/02/skos/core#changeNote> "7/19/24 Merged SKOS entities" .

#################################################################
#    Annotation properties
#################################################################

###  http://www.w3.org/2004/02/skos/core#altLabel
<http://www.w3.org/2004/02/skos/core#altLabel> rdf:type owl:AnnotationProperty ;
                                               rdfs:comment "The range of skos:altLabel is the class of RDF plain literals."@en ,
                                                            "skos:prefLabel, skos:altLabel and skos:hiddenLabel are pairwise disjoint properties."@en ;
                                               rdfs:isDefinedBy <http://www.w3.org/2004/02/skos/core> ;
                                               rdfs:label "alternative label"@en ;
                                               <http://www.w3.org/2004/02/skos/core#definition> "An alternative lexical label for a resource."@en ;
                                               <http://www.w3.org/2004/02/skos/core#example> "Acronyms, abbreviations, spelling variants, and irregular plural/singular forms may be included among the alternative labels for a concept. Mis-spelled terms are normally included as hidden labels (see skos:hiddenLabel)."@en .


###  http://www.w3.org/2004/02/skos/core#changeNote
<http://www.w3.org/2004/02/skos/core#changeNote> rdf:type owl:AnnotationProperty ;
                                                 rdfs:isDefinedBy <http://www.w3.org/2004/02/skos/core> ;
                                                 rdfs:label "change note"@en ;
                                                 <http://www.w3.org/2004/02/skos/core#definition> "A note about a modification to a concept."@en .


###  http://www.w3.org/2004/02/skos/core#definition
<http://www.w3.org/2004/02/skos/core#definition> rdf:type owl:AnnotationProperty ;
                                                 rdfs:isDefinedBy <http://www.w3.org/2004/02/skos/core> ;
                                                 rdfs:label "definition"@en ;
                                                 <http://www.w3.org/2004/02/skos/core#definition> "A statement or formal explanation of the meaning of a concept."@en .


###  http://www.w3.org/2004/02/skos/core#editorialNote
<http://www.w3.org/2004/02/skos/core#editorialNote> rdf:type owl:AnnotationProperty ;
                                                    rdfs:isDefinedBy <http://www.w3.org/2004/02/skos/core> ;
                                                    rdfs:label "editorial note"@en ;
                                                    <http://www.w3.org/2004/02/skos/core#definition> "A note for an editor, translator or maintainer of the vocabulary."@en .


###  http://www.w3.org/2004/02/skos/core#example
<http://www.w3.org/2004/02/skos/core#example> rdf:type owl:AnnotationProperty ;
                                              rdfs:isDefinedBy <http://www.w3.org/2004/02/skos/core> ;
                                              rdfs:label "example"@en ;
                                              <http://www.w3.org/2004/02/skos/core#definition> "An example of the use of a concept."@en .


###  http://www.w3.org/2004/02/skos/core#hiddenLabel
<http://www.w3.org/2004/02/skos/core#hiddenLabel> rdf:type owl:AnnotationProperty ;
                                                  rdfs:comment "The range of skos:hiddenLabel is the class of RDF plain literals."@en ,
                                                               "skos:prefLabel, skos:altLabel and skos:hiddenLabel are pairwise disjoint properties."@en ;
                                                  rdfs:isDefinedBy <http://www.w3.org/2004/02/skos/core> ;
                                                  rdfs:label "hidden label"@en ;
                                                  <http://www.w3.org/2004/02/skos/core#definition> "A lexical label for a resource that should be hidden when generating visual displays of the resource, but should still be accessible to free text search operations."@en .


###  http://www.w3.org/2004/02/skos/core#historyNote
<http://www.w3.org/2004/02/skos/core#historyNote> rdf:type owl:AnnotationProperty ;
                                                  rdfs:isDefinedBy <http://www.w3.org/2004/02/skos/core> ;
                                                  rdfs:label "history note"@en ;
                                                  <http://www.w3.org/2004/02/skos/core#definition> "A note about the past state/use/meaning of a concept."@en .


###  http://www.w3.org/2004/02/skos/core#note
<http://www.w3.org/2004/02/skos/core#note> rdf:type owl:AnnotationProperty ;
                                           rdfs:isDefinedBy <http://www.w3.org/2004/02/skos/core> ;
                                           rdfs:label "note"@en ;
                                           <http://www.w3.org/2004/02/skos/core#definition> "A general note, for any purpose."@en ;
                                           <http://www.w3.org/2004/02/skos/core#scopeNote> "This property may be used directly, or as a super-property for more specific note types."@en .


###  http://www.w3.org/2004/02/skos/core#prefLabel
<http://www.w3.org/2004/02/skos/core#prefLabel> rdf:type owl:AnnotationProperty ;
                                                rdfs:comment "A resource has no more than one value of skos:prefLabel per language tag, and no more than one value of skos:prefLabel without language tag."@en ,
                                                             "The range of skos:prefLabel is the class of RDF plain literals."@en ,
                                                             """skos:prefLabel, skos:altLabel and skos:hiddenLabel are pairwise
      disjoint properties."""@en ;
                                                rdfs:isDefinedBy <http://www.w3.org/2004/02/skos/core> ;
                                                rdfs:label "preferred label"@en ;
                                                <http://www.w3.org/2004/02/skos/core#definition> "The preferred lexical label for a resource, in a given language."@en .


###  http://www.w3.org/2004/02/skos/core#scopeNote
<http://www.w3.org/2004/02/skos/core#scopeNote> rdf:type owl:AnnotationProperty ;
                                                rdfs:isDefinedBy <http://www.w3.org/2004/02/skos/core> ;
                                                rdfs:label "scope note"@en ;
                                                <http://www.w3.org/2004/02/skos/core#definition> "A note that helps to clarify the meaning and/or the use of a concept."@en .


#################################################################
#    Object Properties
#################################################################

###  http://www.semanticweb.org/mdebe/ontologies/2024/6/climatology/addressedBy
:addressedBy rdf:type owl:ObjectProperty ;
             owl:inverseOf :addresses .


###  http://www.semanticweb.org/mdebe/ontologies/2024/6/climatology/addresses
:addresses rdf:type owl:ObjectProperty ;
           rdfs:domain :Project ;
           rdfs:range :Process ;
           rdfs:label "addresses" ;
           <http://www.w3.org/2004/02/skos/core#definition> "The problem or issue that a project addresses" .


###  http://www.semanticweb.org/mdebe/ontologies/2024/6/climatology/contains
:contains rdf:type owl:ObjectProperty ;
          owl:inverseOf :isContainedIn ;
          rdf:type owl:TransitiveProperty ;
          rdfs:domain :Region ;
          rdfs:range :Region ;
          rdfs:label "contains" .


###  http://www.semanticweb.org/mdebe/ontologies/2024/6/climatology/definedQuantitativelyBy
:definedQuantitativelyBy rdf:type owl:ObjectProperty ;
                         rdfs:domain :Climate ;
                         rdfs:range :WeatherElement ;
                         rdfs:label "defined Quantitatively By" .


###  http://www.semanticweb.org/mdebe/ontologies/2024/6/climatology/fundedBy
:fundedBy rdf:type owl:ObjectProperty ;
          owl:inverseOf :funds ;
          rdfs:domain :Project ;
          rdfs:range :Organization ;
          rdfs:label "funded By" ;
          <http://www.w3.org/2004/02/skos/core#definition> "An organization that provides funding for a project" .


###  http://www.semanticweb.org/mdebe/ontologies/2024/6/climatology/funds
:funds rdf:type owl:ObjectProperty ;
       rdfs:label "funds" .


###  http://www.semanticweb.org/mdebe/ontologies/2024/6/climatology/hasLocation
:hasLocation rdf:type owl:ObjectProperty ;
             rdfs:range :Region ;
             rdfs:label "has Location" .


###  http://www.semanticweb.org/mdebe/ontologies/2024/6/climatology/hasPart
:hasPart rdf:type owl:ObjectProperty ;
         owl:inverseOf :isPartOf ;
         rdfs:label "has Part" .


###  http://www.semanticweb.org/mdebe/ontologies/2024/6/climatology/isContainedIn
:isContainedIn rdf:type owl:ObjectProperty ;
               rdfs:subPropertyOf owl:topObjectProperty ;
               rdf:type owl:TransitiveProperty ;
               rdfs:label "is Contained In" .


###  http://www.semanticweb.org/mdebe/ontologies/2024/6/climatology/isPartOf
:isPartOf rdf:type owl:ObjectProperty ;
          rdfs:label "is Part Of" .


###  http://www.semanticweb.org/mdebe/ontologies/2024/6/climatology/sponsoredBy
:sponsoredBy rdf:type owl:ObjectProperty ;
             owl:inverseOf :sponsors ;
             rdfs:domain :Project ;
             rdfs:range :Organization ;
             rdfs:label "sponsored By" ;
             <http://www.w3.org/2004/02/skos/core#definition> "The organization that sponsors (initiates, controls) a project." .


###  http://www.semanticweb.org/mdebe/ontologies/2024/6/climatology/sponsors
:sponsors rdf:type owl:ObjectProperty ;
          rdfs:label "sponsors" .


###  http://www.w3.org/2004/02/skos/core#broadMatch
<http://www.w3.org/2004/02/skos/core#broadMatch> rdf:type owl:ObjectProperty ;
                                                 rdfs:subPropertyOf <http://www.w3.org/2004/02/skos/core#broader> ,
                                                                    <http://www.w3.org/2004/02/skos/core#mappingRelation> ;
                                                 owl:inverseOf <http://www.w3.org/2004/02/skos/core#narrowMatch> ;
                                                 rdfs:isDefinedBy <http://www.w3.org/2004/02/skos/core> ;
                                                 rdfs:label "has broader match"@en ;
                                                 <http://www.w3.org/2004/02/skos/core#definition> "skos:broadMatch is used to state a hierarchical mapping link between two conceptual resources in different concept schemes."@en .


###  http://www.w3.org/2004/02/skos/core#broader
<http://www.w3.org/2004/02/skos/core#broader> rdf:type owl:ObjectProperty ;
                                              rdfs:subPropertyOf <http://www.w3.org/2004/02/skos/core#broaderTransitive> ;
                                              owl:inverseOf <http://www.w3.org/2004/02/skos/core#narrower> ;
                                              rdfs:comment "Broader concepts are typically rendered as parents in a concept hierarchy (tree)."@en ;
                                              rdfs:isDefinedBy <http://www.w3.org/2004/02/skos/core> ;
                                              rdfs:label "has broader"@en ;
                                              <http://www.w3.org/2004/02/skos/core#definition> "Relates a concept to a concept that is more general in meaning."@en ;
                                              <http://www.w3.org/2004/02/skos/core#scopeNote> "By convention, skos:broader is only used to assert an immediate (i.e. direct) hierarchical link between two conceptual resources."@en .


###  http://www.w3.org/2004/02/skos/core#broaderTransitive
<http://www.w3.org/2004/02/skos/core#broaderTransitive> rdf:type owl:ObjectProperty ;
                                                        rdfs:subPropertyOf <http://www.w3.org/2004/02/skos/core#semanticRelation> ;
                                                        owl:inverseOf <http://www.w3.org/2004/02/skos/core#narrowerTransitive> ;
                                                        rdf:type owl:TransitiveProperty ;
                                                        rdfs:isDefinedBy <http://www.w3.org/2004/02/skos/core> ;
                                                        rdfs:label "has broader transitive"@en ;
                                                        <http://www.w3.org/2004/02/skos/core#definition> "skos:broaderTransitive is a transitive superproperty of skos:broader." ;
                                                        <http://www.w3.org/2004/02/skos/core#scopeNote> "By convention, skos:broaderTransitive is not used to make assertions. Rather, the properties can be used to draw inferences about the transitive closure of the hierarchical relation, which is useful e.g. when implementing a simple query expansion algorithm in a search application."@en .


###  http://www.w3.org/2004/02/skos/core#closeMatch
<http://www.w3.org/2004/02/skos/core#closeMatch> rdf:type owl:ObjectProperty ;
                                                 rdfs:subPropertyOf <http://www.w3.org/2004/02/skos/core#mappingRelation> ;
                                                 rdf:type owl:SymmetricProperty ;
                                                 rdfs:isDefinedBy <http://www.w3.org/2004/02/skos/core> ;
                                                 rdfs:label "has close match"@en ;
                                                 <http://www.w3.org/2004/02/skos/core#definition> "skos:closeMatch is used to link two concepts that are sufficiently similar that they can be used interchangeably in some information retrieval applications. In order to avoid the possibility of \"compound errors\" when combining mappings across more than two concept schemes, skos:closeMatch is not declared to be a transitive property."@en .


###  http://www.w3.org/2004/02/skos/core#exactMatch
<http://www.w3.org/2004/02/skos/core#exactMatch> rdf:type owl:ObjectProperty ;
                                                 rdfs:subPropertyOf <http://www.w3.org/2004/02/skos/core#closeMatch> ;
                                                 rdf:type owl:SymmetricProperty ,
                                                          owl:TransitiveProperty ;
                                                 rdfs:comment "skos:exactMatch is disjoint with each of the properties skos:broadMatch and skos:relatedMatch."@en ;
                                                 rdfs:isDefinedBy <http://www.w3.org/2004/02/skos/core> ;
                                                 rdfs:label "has exact match"@en ;
                                                 <http://www.w3.org/2004/02/skos/core#definition> "skos:exactMatch is used to link two concepts, indicating a high degree of confidence that the concepts can be used interchangeably across a wide range of information retrieval applications. skos:exactMatch is a transitive property, and is a sub-property of skos:closeMatch."@en .


###  http://www.w3.org/2004/02/skos/core#hasTopConcept
<http://www.w3.org/2004/02/skos/core#hasTopConcept> rdf:type owl:ObjectProperty ;
                                                    owl:inverseOf <http://www.w3.org/2004/02/skos/core#topConceptOf> ;
                                                    rdfs:domain <http://www.w3.org/2004/02/skos/core#ConceptScheme> ;
                                                    rdfs:range <http://www.w3.org/2004/02/skos/core#Concept> ;
                                                    rdfs:isDefinedBy <http://www.w3.org/2004/02/skos/core> ;
                                                    rdfs:label "has top concept"@en ;
                                                    <http://www.w3.org/2004/02/skos/core#definition> "Relates, by convention, a concept scheme to a concept which is topmost in the broader/narrower concept hierarchies for that scheme, providing an entry point to these hierarchies."@en .


###  http://www.w3.org/2004/02/skos/core#inScheme
<http://www.w3.org/2004/02/skos/core#inScheme> rdf:type owl:ObjectProperty ;
                                               rdfs:range <http://www.w3.org/2004/02/skos/core#ConceptScheme> ;
                                               rdfs:comment "This property and its sub-properties are from SKOS. They may be useful in the future for modeling concepts that are difficult to define or that come from other knowledge structures such as Taxonomies that don't follow OWL semantic. M DeBellis 7/24/24" ;
                                               rdfs:isDefinedBy <http://www.w3.org/2004/02/skos/core> ;
                                               rdfs:label "is in scheme"@en ;
                                               <http://www.w3.org/2004/02/skos/core#definition> "Relates a resource (for example a concept) to a concept scheme in which it is included."@en ;
                                               <http://www.w3.org/2004/02/skos/core#scopeNote> "A concept may be a member of more than one concept scheme."@en .


###  http://www.w3.org/2004/02/skos/core#mappingRelation
<http://www.w3.org/2004/02/skos/core#mappingRelation> rdf:type owl:ObjectProperty ;
                                                      rdfs:subPropertyOf <http://www.w3.org/2004/02/skos/core#semanticRelation> ;
                                                      rdfs:comment "These concept mapping relations mirror semantic relations, and the data model defined below is similar (with the exception of skos:exactMatch) to the data model defined for semantic relations. A distinct vocabulary is provided for concept mapping relations, to provide a convenient way to differentiate links within a concept scheme from links between concept schemes. However, this pattern of usage is not a formal requirement of the SKOS data model, and relies on informal definitions of best practice."@en ;
                                                      rdfs:isDefinedBy <http://www.w3.org/2004/02/skos/core> ;
                                                      rdfs:label "is in mapping relation with"@en ;
                                                      <http://www.w3.org/2004/02/skos/core#definition> "Relates two concepts coming, by convention, from different schemes, and that have comparable meanings"@en .


###  http://www.w3.org/2004/02/skos/core#narrowMatch
<http://www.w3.org/2004/02/skos/core#narrowMatch> rdf:type owl:ObjectProperty ;
                                                  rdfs:subPropertyOf <http://www.w3.org/2004/02/skos/core#mappingRelation> ,
                                                                     <http://www.w3.org/2004/02/skos/core#narrower> ;
                                                  rdfs:isDefinedBy <http://www.w3.org/2004/02/skos/core> ;
                                                  rdfs:label "has narrower match"@en ;
                                                  <http://www.w3.org/2004/02/skos/core#definition> "skos:narrowMatch is used to state a hierarchical mapping link between two conceptual resources in different concept schemes."@en .


###  http://www.w3.org/2004/02/skos/core#narrower
<http://www.w3.org/2004/02/skos/core#narrower> rdf:type owl:ObjectProperty ;
                                               rdfs:subPropertyOf <http://www.w3.org/2004/02/skos/core#narrowerTransitive> ;
                                               rdfs:comment "Narrower concepts are typically rendered as children in a concept hierarchy (tree)."@en ;
                                               rdfs:isDefinedBy <http://www.w3.org/2004/02/skos/core> ;
                                               rdfs:label "has narrower"@en ;
                                               <http://www.w3.org/2004/02/skos/core#definition> "Relates a concept to a concept that is more specific in meaning."@en ;
                                               <http://www.w3.org/2004/02/skos/core#scopeNote> "By convention, skos:broader is only used to assert an immediate (i.e. direct) hierarchical link between two conceptual resources."@en .


###  http://www.w3.org/2004/02/skos/core#narrowerTransitive
<http://www.w3.org/2004/02/skos/core#narrowerTransitive> rdf:type owl:ObjectProperty ;
                                                         rdfs:subPropertyOf <http://www.w3.org/2004/02/skos/core#semanticRelation> ;
                                                         rdf:type owl:TransitiveProperty ;
                                                         rdfs:isDefinedBy <http://www.w3.org/2004/02/skos/core> ;
                                                         rdfs:label "has narrower transitive"@en ;
                                                         <http://www.w3.org/2004/02/skos/core#definition> "skos:narrowerTransitive is a transitive superproperty of skos:narrower." ;
                                                         <http://www.w3.org/2004/02/skos/core#scopeNote> "By convention, skos:narrowerTransitive is not used to make assertions. Rather, the properties can be used to draw inferences about the transitive closure of the hierarchical relation, which is useful e.g. when implementing a simple query expansion algorithm in a search application."@en .


###  http://www.w3.org/2004/02/skos/core#related
<http://www.w3.org/2004/02/skos/core#related> rdf:type owl:ObjectProperty ;
                                              rdfs:subPropertyOf <http://www.w3.org/2004/02/skos/core#semanticRelation> ;
                                              rdf:type owl:SymmetricProperty ;
                                              rdfs:comment "skos:related is disjoint with skos:broaderTransitive"@en ;
                                              rdfs:isDefinedBy <http://www.w3.org/2004/02/skos/core> ;
                                              rdfs:label "has related"@en ;
                                              <http://www.w3.org/2004/02/skos/core#definition> "Relates a concept to a concept with which there is an associative semantic relationship."@en .


###  http://www.w3.org/2004/02/skos/core#relatedMatch
<http://www.w3.org/2004/02/skos/core#relatedMatch> rdf:type owl:ObjectProperty ;
                                                   rdfs:subPropertyOf <http://www.w3.org/2004/02/skos/core#mappingRelation> ,
                                                                      <http://www.w3.org/2004/02/skos/core#related> ;
                                                   rdf:type owl:SymmetricProperty ;
                                                   rdfs:isDefinedBy <http://www.w3.org/2004/02/skos/core> ;
                                                   rdfs:label "has related match"@en ;
                                                   <http://www.w3.org/2004/02/skos/core#definition> "skos:relatedMatch is used to state an associative mapping link between two conceptual resources in different concept schemes."@en .


###  http://www.w3.org/2004/02/skos/core#semanticRelation
<http://www.w3.org/2004/02/skos/core#semanticRelation> rdf:type owl:ObjectProperty ;
                                                       rdfs:domain <http://www.w3.org/2004/02/skos/core#Concept> ;
                                                       rdfs:range <http://www.w3.org/2004/02/skos/core#Concept> ;
                                                       rdfs:comment "This property and its sub-properties are from SKOS. They may be useful in the future for modeling concepts that are difficult to define or that come from other knowledge structures such as Taxonomies that don't follow OWL semantic. M DeBellis 7/24/24" ;
                                                       rdfs:isDefinedBy <http://www.w3.org/2004/02/skos/core> ;
                                                       rdfs:label "is in semantic relation with"@en ;
                                                       <http://www.w3.org/2004/02/skos/core#definition> "Links a concept to a concept related by meaning."@en ;
                                                       <http://www.w3.org/2004/02/skos/core#scopeNote> "This property should not be used directly, but as a super-property for all properties denoting a relationship of meaning between concepts."@en .


###  http://www.w3.org/2004/02/skos/core#topConceptOf
<http://www.w3.org/2004/02/skos/core#topConceptOf> rdf:type owl:ObjectProperty ;
                                                   rdfs:subPropertyOf <http://www.w3.org/2004/02/skos/core#inScheme> ;
                                                   rdfs:domain <http://www.w3.org/2004/02/skos/core#Concept> ;
                                                   rdfs:range <http://www.w3.org/2004/02/skos/core#ConceptScheme> ;
                                                   rdfs:isDefinedBy <http://www.w3.org/2004/02/skos/core> ;
                                                   rdfs:label "is top concept in scheme"@en ;
                                                   <http://www.w3.org/2004/02/skos/core#definition> "Relates a concept to the concept scheme that it is a top level concept of."@en .


#################################################################
#    Data properties
#################################################################

###  http://www.semanticweb.org/mdebe/ontologies/2024/6/climatology/atmosphericHumidity
:atmosphericHumidity rdf:type owl:DatatypeProperty ;
                     rdfs:subPropertyOf :regionProperty ;
                     <http://www.w3.org/2004/02/skos/core#definition> """Atmospheric humidity is the amount of water vapor carried in the air. It can be measured as vapor pressure, mixing ratio or specific humidity. Specific humidity is the ratio of vapor mass to total air mass, whereas mixing ratio is the ratio of the mass of vapor to the mass of dry air. The atmosphere must carry away the water evaporated from the surface and supply water to areas of rainfall. Water that flows from the land to the oceans in rivers was brought to the land areas by transport in the atmosphere as vapor. Atmospheric water vapor is also the most important greenhouse gas in the atmosphere. Water vapor condenses to form clouds, which can release rainfall and are also extremely important in both reflecting solar radiation and reducing the infrared radiation emitted by Earth.

Hartmann, Dennis L. (2015-12-02T22:58:59.000). Global Physical Climatology . Elsevier Science. Kindle Edition.""" .


###  http://www.semanticweb.org/mdebe/ontologies/2024/6/climatology/climateVariable
:climateVariable rdf:type owl:DatatypeProperty ,
                          owl:FunctionalProperty ;
                 rdfs:domain :Climate .


###  http://www.semanticweb.org/mdebe/ontologies/2024/6/climatology/latitude
:latitude rdf:type owl:DatatypeProperty ;
          rdfs:subPropertyOf :regionProperty .


###  http://www.semanticweb.org/mdebe/ontologies/2024/6/climatology/longitude
:longitude rdf:type owl:DatatypeProperty ;
           rdfs:subPropertyOf :regionProperty .


###  http://www.semanticweb.org/mdebe/ontologies/2024/6/climatology/precipitation
:precipitation rdf:type owl:DatatypeProperty ;
               rdfs:subPropertyOf :climateVariable ,
                                  :regionProperty .


###  http://www.semanticweb.org/mdebe/ontologies/2024/6/climatology/regionProperty
:regionProperty rdf:type owl:DatatypeProperty ;
                rdfs:domain :Region .


###  http://www.semanticweb.org/mdebe/ontologies/2024/6/climatology/temperature
:temperature rdf:type owl:DatatypeProperty ;
             rdfs:subPropertyOf :climateVariable ,
                                :regionProperty .


###  http://www.w3.org/2004/02/skos/core#notation
<http://www.w3.org/2004/02/skos/core#notation> rdf:type owl:DatatypeProperty ;
                                               rdfs:isDefinedBy <http://www.w3.org/2004/02/skos/core> ;
                                               rdfs:label "notation"@en ;
                                               <http://www.w3.org/2004/02/skos/core#definition> "A notation, also known as classification code, is a string of characters such as \"T58.5\" or \"303.4833\" used to uniquely identify a concept within the scope of a given concept scheme."@en ;
                                               <http://www.w3.org/2004/02/skos/core#scopeNote> "By convention, skos:notation is used with a typed literal in the object position of the triple."@en .


#################################################################
#    Classes
#################################################################

###  http://www.semanticweb.org/mdebe/ontologies/2024/6/climatology/AdiabaticProcess
:AdiabaticProcess rdf:type owl:Class ;
                  rdfs:subClassOf :Process ;
                  rdfs:label "Adiabatic Process" ;
                  <http://www.w3.org/2004/02/skos/core#definition> """An adiabatic process is one for which no heat is added or taken away so, δQ = 0, and (1.17) can be rearranged to read, so that for a parcel of gas that undergoes an adiabatic process, (1.19) If we define Θ to be the temperature at some reference pressure po, which is usually taken to be 1000 hPa, then the potential temperature Θ is the temperature a parcel of air would have if it were brought adiabatically to the reference pressure. (1.20)

Hartmann, Dennis L. (2015-12-02T22:58:59.000). Global Physical Climatology . Elsevier Science. Kindle Edition.""" .


###  http://www.semanticweb.org/mdebe/ontologies/2024/6/climatology/Agent
:Agent rdf:type owl:Class ;
       rdfs:label "Agent" .


###  http://www.semanticweb.org/mdebe/ontologies/2024/6/climatology/City
:City rdf:type owl:Class ;
      rdfs:subClassOf :Region ;
      rdfs:label "City" .


###  http://www.semanticweb.org/mdebe/ontologies/2024/6/climatology/Climate
:Climate rdf:type owl:Class ;
         owl:equivalentClass [ rdf:type owl:Restriction ;
                               owl:onProperty :definedQuantitativelyBy ;
                               owl:someValuesFrom :WeatherElement
                             ] ;
         rdfs:subClassOf :ClimateSystem ;
         rdfs:label "Climate" ;
         <http://www.w3.org/2004/02/skos/core#definition> """Climate is the synthesis of the weather in a particular region. It can be defined quantitatively by using the expected values of the meteorological elements at a location during a certain month or season. The expected values of the meteorological elements can be called the climatic elements and include variables such as the average temperature, precipitation, wind, pressure, cloudiness, and humidity. In defining the climate, we usually employ the values of these elements at the surface of Earth. Thus, one can characterize the climate of Seattle by stating that the average annual mean precipitation is 38 in. and the annual mean temperature is 52°F. However, one might need a great deal more information than the annual means. For example, a farmer would also like to know how the precipitation is distributed through the year and how much rain would fall during the critical summer months. A hydroelectric plant engineer needs to know how much interannual variability in rainfall and snow accumulation to expect. A homebuilder should know how much insulation to be installed and the size of the heating or cooling unit needed to provide for the weather in the region. Sailors might like to know that the wind blows in the winter, but not so much in the summer. The importance of climate is so basic that we sometimes overlook it. If the climate were not more or less as it is, life and civilization on this planet would not have developed as they have. The distribution of vegetation and soil type over the land areas is determined primarily by the local climate. Climate affects human lives in many ways; for example, climate influences the type of clothing and housing that people have developed. In the modern world, with the great technological advances of the past century, one might think that climate no longer constitutes a force capable of changing the course of human history. It is apparent, on the contrary, that we are as sensitive now as we have ever been to climate fluctuations and climate change.

Hartmann, Dennis L. (2015-12-02T22:58:59.000). Global Physical Climatology . Elsevier Science. Kindle Edition. .""" .


###  http://www.semanticweb.org/mdebe/ontologies/2024/6/climatology/ClimateSystem
:ClimateSystem rdf:type owl:Class ;
               rdfs:label "Climate System" .


###  http://www.semanticweb.org/mdebe/ontologies/2024/6/climatology/ClimaticAnalomy
:ClimaticAnalomy rdf:type owl:Class ;
                 rdfs:subClassOf :Climate ;
                 rdfs:label "Climatic Analomy" ;
                 <http://www.w3.org/2004/02/skos/core#definition> """Because food, water, and energy supply systems are strained to meet demand and are optimized to the current average climatic conditions, fluctuations or trends in climate can cause serious difficulties for humanity. Moreover, since the population has grown to absorb the maximum agricultural productivity in much of the world, the absolute number of human lives at risk of starvation during climatic anomalies has never been greater. In addition to natural year-to-year fluctuations in the weather, which are an important aspect of climate, we must be concerned with the effects of human activities in producing long-term trends in the climate. It is now clear that humans are affecting the global climate, and this influence is growing.

Hartmann, Dennis L. (2015-12-02T22:58:59.000). Global Physical Climatology . Elsevier Science. Kindle Edition.""" .


###  http://www.semanticweb.org/mdebe/ontologies/2024/6/climatology/Corporation
:Corporation rdf:type owl:Class ;
             rdfs:subClassOf :Organization ;
             rdfs:label "Corporation" .


###  http://www.semanticweb.org/mdebe/ontologies/2024/6/climatology/District
:District rdf:type owl:Class ;
          rdfs:subClassOf :Region ;
          rdfs:label "District" .


###  http://www.semanticweb.org/mdebe/ontologies/2024/6/climatology/Government
:Government rdf:type owl:Class ;
            rdfs:subClassOf :Organization ;
            rdfs:label "Government" .


###  http://www.semanticweb.org/mdebe/ontologies/2024/6/climatology/Group
:Group rdf:type owl:Class ;
       rdfs:subClassOf :Agent ;
       rdfs:label "Group" .


###  http://www.semanticweb.org/mdebe/ontologies/2024/6/climatology/HighTideFloodingAndShorelineErosion
:HighTideFloodingAndShorelineErosion rdf:type owl:Class ;
                                     rdfs:subClassOf :ProcessInfluencedByClimateChange ;
                                     rdfs:label "High Tide Flooding And Shoreline Erosion" .


###  http://www.semanticweb.org/mdebe/ontologies/2024/6/climatology/Humidity
:Humidity rdf:type owl:Class ;
          rdfs:subClassOf :WeatherElement ;
          rdfs:label "Humidity" ;
          <http://www.w3.org/2004/02/skos/core#definition> """The humidity, the amount of water vapor in the air, is a critical climate factor that is related closely to the temperature and precipitation.

Hartmann, Dennis L. (2015-12-02T22:58:59.000). Global Physical Climatology . Elsevier Science. Kindle Edition.""" .


###  http://www.semanticweb.org/mdebe/ontologies/2024/6/climatology/Nation
:Nation rdf:type owl:Class ;
        rdfs:subClassOf :Region ;
        rdfs:label "Nation" .


###  http://www.semanticweb.org/mdebe/ontologies/2024/6/climatology/NonGovernmentalOrganization
:NonGovernmentalOrganization rdf:type owl:Class ;
                             rdfs:subClassOf :Organization ;
                             rdfs:label "Non Governmental Organization" .


###  http://www.semanticweb.org/mdebe/ontologies/2024/6/climatology/Organization
:Organization rdf:type owl:Class ;
              rdfs:subClassOf :Group ;
              rdfs:label "Organization" .


###  http://www.semanticweb.org/mdebe/ontologies/2024/6/climatology/Precipitation
:Precipitation rdf:type owl:Class ;
               rdfs:subClassOf :WeatherElement ;
               rdfs:label "Precipitation" .


###  http://www.semanticweb.org/mdebe/ontologies/2024/6/climatology/Process
:Process rdf:type owl:Class ;
         rdfs:label "Process" .


###  http://www.semanticweb.org/mdebe/ontologies/2024/6/climatology/ProcessInfluencedByClimateChange
:ProcessInfluencedByClimateChange rdf:type owl:Class ;
                                  rdfs:subClassOf :Process ;
                                  rdfs:label "Process Influenced By Climate Change" .


###  http://www.semanticweb.org/mdebe/ontologies/2024/6/climatology/Project
:Project rdf:type owl:Class ;
         rdfs:subClassOf :Process ;
         rdfs:label "Project" .


###  http://www.semanticweb.org/mdebe/ontologies/2024/6/climatology/Province
:Province rdf:type owl:Class ;
          rdfs:subClassOf :Region ;
          rdfs:label "Province" .


###  http://www.semanticweb.org/mdebe/ontologies/2024/6/climatology/Region
:Region rdf:type owl:Class ;
        rdfs:subClassOf :ClimateSystem ;
        rdfs:label "Region" ;
        <http://www.w3.org/2004/02/skos/core#definition> "Climate is the synthesis of the weather in a particular region. It can be defined quantitatively by using the expected values of the meteorological elements at a location during a certain month or season." .


###  http://www.semanticweb.org/mdebe/ontologies/2024/6/climatology/State
:State rdf:type owl:Class ;
       rdfs:subClassOf :Region ;
       rdfs:label "State" .


###  http://www.semanticweb.org/mdebe/ontologies/2024/6/climatology/Temperature
:Temperature rdf:type owl:Class ;
             rdfs:subClassOf :WeatherElement ;
             rdfs:label "Temperature" .


###  http://www.semanticweb.org/mdebe/ontologies/2024/6/climatology/Village
:Village rdf:type owl:Class ;
         rdfs:subClassOf :Region ;
         rdfs:label "Village" .


###  http://www.semanticweb.org/mdebe/ontologies/2024/6/climatology/WeatherElement
:WeatherElement rdf:type owl:Class ;
                rdfs:subClassOf :ClimateSystem ;
                rdfs:label "Weather Element" ;
                <http://www.w3.org/2004/02/skos/core#definition> """The climate of Earth is defined in terms of measurable weather elements. The weather elements of most interest are temperature and precipitation. These two factors together largely determine the species of plants and animals that survive and prosper in a particular location. Other variables are also important, of course. The humidity, the amount of water vapor in the air, is a critical climate factor that is related closely to the temperature and precipitation. Condensation of water in the atmosphere produces clouds of water droplets or ice particles that greatly change the radiative properties of the atmosphere.

Hartmann, Dennis L. (2015-12-02T22:58:59.000). Global Physical Climatology . Elsevier Science. Kindle Edition.""" .


###  http://www.w3.org/2004/02/skos/core#Concept
<http://www.w3.org/2004/02/skos/core#Concept> rdf:type owl:Class ;
                                              owl:disjointWith <http://www.w3.org/2004/02/skos/core#ConceptScheme> ;
                                              rdfs:comment "This class is from SKOS. They may be useful in the future for modeling concepts that are difficult to define or that come from other knowledge structures such as Taxonomies that don't follow OWL semantic. M DeBellis 7/24/24" ;
                                              rdfs:isDefinedBy <http://www.w3.org/2004/02/skos/core> ;
                                              rdfs:label "Concept"@en ;
                                              <http://www.w3.org/2004/02/skos/core#definition> "An idea or notion; a unit of thought."@en .


###  http://www.w3.org/2004/02/skos/core#ConceptScheme
<http://www.w3.org/2004/02/skos/core#ConceptScheme> rdf:type owl:Class ;
                                                    rdfs:comment "This class is from SKOS. They may be useful in the future for modeling concepts that are difficult to define or that come from other knowledge structures such as Taxonomies that don't follow OWL semantic. M DeBellis 7/24/24" ;
                                                    rdfs:isDefinedBy <http://www.w3.org/2004/02/skos/core> ;
                                                    rdfs:label "Concept Scheme"@en ;
                                                    <http://www.w3.org/2004/02/skos/core#definition> "A set of concepts, optionally including statements about semantic relationships between those concepts."@en ;
                                                    <http://www.w3.org/2004/02/skos/core#example> "Thesauri, classification schemes, subject heading lists, taxonomies, 'folksonomies', and other types of controlled vocabulary are all examples of concept schemes. Concept schemes are also embedded in glossaries and terminologies."@en ;
                                                    <http://www.w3.org/2004/02/skos/core#scopeNote> "A concept scheme may be defined to include concepts from different sources."@en .


#################################################################
#    Individuals
#################################################################

###  http://www.semanticweb.org/mdebe/ontologies/2024/6/climatology/Alabama
:Alabama rdf:type owl:NamedIndividual ,
                  :State ;
         rdfs:label "Alabama" .


###  http://www.semanticweb.org/mdebe/ontologies/2024/6/climatology/California
:California rdf:type owl:NamedIndividual ,
                     :State ;
            :contains :SanFrancisco ;
            rdfs:label "California" .


###  http://www.semanticweb.org/mdebe/ontologies/2024/6/climatology/Chicago
:Chicago rdf:type owl:NamedIndividual ,
                  :City ;
         rdfs:label "Chicago" .


###  http://www.semanticweb.org/mdebe/ontologies/2024/6/climatology/ClimatrOfSeattle
:ClimatrOfSeattle rdf:type owl:NamedIndividual ;
                  rdfs:label "Climatr Of Seattle" .


###  http://www.semanticweb.org/mdebe/ontologies/2024/6/climatology/Cryosphere
:Cryosphere rdf:type owl:NamedIndividual ,
                     :Region ;
            rdfs:label "Cryosphere" ;
            <http://www.w3.org/2004/02/skos/core#definition> """All of the ice near the surface of Earth is called the cryosphere. About 2% of the water on Earth is frozen, and this frozen water constitutes about 80% of the freshwater. Most of the mass of ice is contained in the great ice sheets of Antarctica (89%) and Greenland (8.6%) (Table 1.4). For climate, it is often not the mass of ice that is of primary importance, but rather the surface area that is covered by ice of any depth. This is because surface ice of any depth generally is a much more effective reflector of solar radiation than the underlying surface. Also, sea ice is a good insulator and allows air temperature to be very different from that of the seawater under just a few meters of sea ice. Currently, year-round (perennial) ice covers about 11% of the land area and 7% of the world ocean. During some seasons, the amount of land covered by seasonal snow cover exceeds the surface area covered by perennial ice cover. The surface areas covered by ice sheets, seasonal snow, and sea ice are comparable. Ice sheets cover about 16 × 106 km2, seasonal snow about 50 × 106 km2, and sea ice up to 23 × 106 km2.

Hartmann, Dennis L. (2015-12-02T22:58:59.000). Global Physical Climatology . Elsevier Science. Kindle Edition.""" .


###  http://www.semanticweb.org/mdebe/ontologies/2024/6/climatology/Earth
:Earth rdf:type owl:NamedIndividual ,
                :Region ;
       :contains :TheLandSurface ,
                 :TheWorldOcean ;
       rdfs:label "Earth" .


###  http://www.semanticweb.org/mdebe/ontologies/2024/6/climatology/FirstLawOfThermodynaims
:FirstLawOfThermodynaims rdf:type owl:NamedIndividual ,
                                  :Process ;
                         rdfs:label "First Law Of Thermodynaims" ;
                         <http://www.w3.org/2004/02/skos/core#definition> """The first law of thermodynamics states that energy is conserved, so that for a unit mass of gas, the applied heat δQ is equal to the sum of the change in internal energy dU and the work done dW. If we assume that the external work done by air is only that associated with volume changes, dW = pdα, and we use the definition of the specific heat at constant volume , we obtain a useful form of the first law of thermodynamics. (1.12) Here p is pressure, dT is the change in temperature, and dα is the change in specific volume, α. Using the ideal gas law, (1.13) we may write that,(1.15) (1.12) becomes, (1.16) or using (1.13) again, (1.17)

Hartmann, Dennis L. (2015-12-02T22:58:59.000). Global Physical Climatology . Elsevier Science. Kindle Edition.""" .


###  http://www.semanticweb.org/mdebe/ontologies/2024/6/climatology/GlobalClimateChange
:GlobalClimateChange rdf:type owl:NamedIndividual ,
                              :ClimaticAnalomy ;
                     :hasLocation :Earth ;
                     rdfs:label "Global Climate Change" .


###  http://www.semanticweb.org/mdebe/ontologies/2024/6/climatology/High-TideFloodingAndShorelineErosionInNorfolkVirginia
:High-TideFloodingAndShorelineErosionInNorfolkVirginia rdf:type owl:NamedIndividual ,
                                                                :HighTideFloodingAndShorelineErosion ;
                                                       :hasLocation :Norfolk ;
                                                       rdfs:label "High-Tide Flooding And Shoreline Erosion In Norfolk Virginia" ;
                                                       <http://www.w3.org/2004/02/skos/core#definition> "Norfolk, Virginia, is experiencing some of the highest rates of sea level rise in the nation. Rising sea levels threaten neighborhoods, public infrastructure, and historical sites." .


###  http://www.semanticweb.org/mdebe/ontologies/2024/6/climatology/HydrostaticBalance
:HydrostaticBalance rdf:type owl:NamedIndividual ,
                             :Process ;
                    rdfs:label "Hydrostatic Balance" ;
                    <http://www.w3.org/2004/02/skos/core#definition> """The atmosphere is composed of gases held close to the surface of the planet by gravity. The vertical forces acting on the atmosphere at rest are gravity, which pulls the air molecules toward the center of the planet, and the pressure gradient force, which tries to push the atmosphere out into space. These forces are in balance to a very good approximation, and by equating the pressure gradient force and the gravity force one obtains the hydrostatic balance. Since force is mass times acceleration, we may express the vertical force balance per unit mass as an equation between the downward acceleration of gravity, g, and the upward acceleration that would be caused by the increase of pressure toward the ground, if gravity were not present to oppose it. (1.2) For an ideal gas, pressure (p), density (ρ), and temperature (T) are related by the formula (1.3) where R is the gas constant. After some rearrangement, (1.2) and (1.3) yield (1.4) where

Hartmann, Dennis L. (2015-12-02T22:58:59.000). Global Physical Climatology . Elsevier Science. Kindle Edition.""" .


###  http://www.semanticweb.org/mdebe/ontologies/2024/6/climatology/Illinois
:Illinois rdf:type owl:NamedIndividual ,
                   :State ;
          :contains :Chicago ;
          rdfs:label "Illinois" .


###  http://www.semanticweb.org/mdebe/ontologies/2024/6/climatology/India
:India rdf:type owl:NamedIndividual ,
                :Nation ;
       rdfs:label "India" .


###  http://www.semanticweb.org/mdebe/ontologies/2024/6/climatology/InflationReductionAct
:InflationReductionAct rdf:type owl:NamedIndividual ,
                                :Project ;
                       :addresses :GlobalClimateChange ;
                       :fundedBy :USFederalGovernment ;
                       :sponsoredBy :USFederalGovernment ;
                       rdfs:label "Inflation Reduction Act" ;
                       <http://www.w3.org/2004/02/skos/core#definition> """President Biden’s Climate Initiatives: The Inflation Reduction Act (IRA):
President Biden and Congress have taken  steps to combat the climate crisis.
The IRA aims to reduce inflation while also addressing climate change and improving energy security.""" .


###  http://www.semanticweb.org/mdebe/ontologies/2024/6/climatology/Norfolk
:Norfolk rdf:type owl:NamedIndividual ,
                  :City ;
         rdfs:label "Norfolk" .


###  http://www.semanticweb.org/mdebe/ontologies/2024/6/climatology/NorfolkCityGovernment
:NorfolkCityGovernment rdf:type owl:NamedIndividual ,
                                :Government ;
                       :hasLocation :Norfolk ;
                       rdfs:label "Norfolk City Government" .


###  http://www.semanticweb.org/mdebe/ontologies/2024/6/climatology/OhioCreekWatershedProject
:OhioCreekWatershedProject rdf:type owl:NamedIndividual ,
                                    :Project ;
                           :addresses :High-TideFloodingAndShorelineErosionInNorfolkVirginia ;
                           :fundedBy :USFederalGovernment ;
                           :sponsoredBy :NorfolkCityGovernment ;
                           rdfs:label "Ohio Creek Watershed Project" .


###  http://www.semanticweb.org/mdebe/ontologies/2024/6/climatology/SanFrancisco
:SanFrancisco rdf:type owl:NamedIndividual ,
                       :City ;
              rdfs:label "San Francisco" .


###  http://www.semanticweb.org/mdebe/ontologies/2024/6/climatology/Seattle
:Seattle rdf:type owl:NamedIndividual ,
                  :City ;
         rdfs:label "Seattle" .


###  http://www.semanticweb.org/mdebe/ontologies/2024/6/climatology/TheLandSurface
:TheLandSurface rdf:type owl:NamedIndividual ,
                         :Region ;
                :contains :India ,
                          :UK ,
                          :USA ;
                rdfs:label "The Land Surface" ;
                <http://www.w3.org/2004/02/skos/core#definition> """Although the land surface covers only 29% of Earth, the climate over the land surface is extremely important to us because humans are land-dwelling creatures. Cereal grains are the world’s most important food source, and supply about half of the world’s calories and muchof the protein. About 80% of the animal protein consumed by humans comes from meat, eggs, and dairy products, and only 20% from seafood. Over the land surface, temperature and soil moisture are key determinants of natural vegetation and the agricultural potential of a given area. Vegetation, snow cover, and soil conditions also affect the local and global climate, so that local climate and land surface conditions participate in a two-way relationship. Land topography plays an important role in modifying regional climates, and weathering of rocks on land is a key component of the carbon cycle that controls the carbon dioxide content of the atmosphere on millennial time scales. The arrangement of land and ocean areas on Earth plays a role in determining global climate. The arrangement of land and ocean varies on time scales of millions of years as the continents drift about. At the present time, about 68% of Earth’s land area is in the Northern Hemisphere (Fig. 1.13). The fact that the Northern Hemisphere has most of the land area causes significant differences in the climates of the Northern and Southern Hemispheres, and plays an important role in climate change. The Northern Hemisphere has much more dramatic east–west variations in continental elevation, especially in middle latitudes where the Himalaya and Rocky Mountains are prominent features (Fig. 1.14). The topography of the land surface and the arrangement and orientation of mountain ranges are key determinants of climate.

Hartmann, Dennis L. (2015-12-02T22:58:59.000). Global Physical Climatology . Elsevier Science. Kindle Edition.""" .


###  http://www.semanticweb.org/mdebe/ontologies/2024/6/climatology/TheWorldOcean
:TheWorldOcean rdf:type owl:NamedIndividual ,
                        :Region ;
               rdfs:label "The World Ocean" .


###  http://www.semanticweb.org/mdebe/ontologies/2024/6/climatology/UK
:UK rdf:type owl:NamedIndividual ,
             :Nation ;
    rdfs:label "U K" .


###  http://www.semanticweb.org/mdebe/ontologies/2024/6/climatology/USA
:USA rdf:type owl:NamedIndividual ,
              :Nation ;
     :contains :Alabama ,
               :California ,
               :Washington ;
     rdfs:label "U S A" .


###  http://www.semanticweb.org/mdebe/ontologies/2024/6/climatology/USFederalGovernment
:USFederalGovernment rdf:type owl:NamedIndividual ,
                              :Government ;
                     rdfs:label "U S Federal Government" .


###  http://www.semanticweb.org/mdebe/ontologies/2024/6/climatology/Virginia
:Virginia rdf:type owl:NamedIndividual ,
                   :State ;
          :contains :Norfolk ;
          rdfs:label "Virginia" .


###  http://www.semanticweb.org/mdebe/ontologies/2024/6/climatology/Washington
:Washington rdf:type owl:NamedIndividual ,
                     :State ;
            :contains :Seattle ;
            rdfs:label "Washington" .


#################################################################
#    Annotations
#################################################################

:Oregon rdfs:label "Oregon" .


#################################################################
#    General axioms
#################################################################

[ rdf:type owl:AllDisjointClasses ;
  owl:members ( :City
                :District
                :Nation
                :Province
                :State
                :Village
              )
] .


[ rdf:type owl:AllDisjointClasses ;
  owl:members ( :Corporation
                :Government
                :NonGovernmentalOrganization
              )
] .


###  Generated by the OWL API (version 4.5.29.2024-05-13T12:11:03Z) https://github.com/owlcs/owlapi
